rename RE, REAns to RPre, RPost

theories/Automation.v
@@ -13,215 +13,215 @@ Local Open Scope monad_scope.
 
 (** * Basic Refinement Lemmas *)
 
-Lemma padded_refines_ret E1 E2 R1 R2 RE REAns RR r1 r2 :
+Lemma padded_refines_ret E1 E2 R1 R2 RPre RPost RR r1 r2 :
   (RR r1 r2 : Prop) ->
-  @padded_refines E1 E2 R1 R2 RE REAns RR (Ret r1) (Ret r2).
+  @padded_refines E1 E2 R1 R2 RPre RPost RR (Ret r1) (Ret r2).
 Proof.
   apply padded_refines_ret.
 Qed.
 
 Lemma padded_refines_vis E1 E2 R1 R2 A B
-        RE REAns RR (e1 : E1 A) (e2 : E2 B)
+        RPre RPost RR (e1 : E1 A) (e2 : E2 B)
         (k1 : A -> itree_spec E1 R1) (k2 : B -> itree_spec E2 R2) :
-  (RE A B e1 e2 : Prop) ->
-  (forall a b, (REAns A B e1 e2 a b : Prop) -> padded_refines RE REAns RR (k1 a) (k2 b)) ->
-  padded_refines RE REAns RR (Vis (Spec_vis e1) k1) (Vis (Spec_vis e2) k2).
+  (RPre A B e1 e2 : Prop) ->
+  (forall a b, (RPost A B e1 e2 a b : Prop) -> padded_refines RPre RPost RR (k1 a) (k2 b)) ->
+  padded_refines RPre RPost RR (Vis (Spec_vis e1) k1) (Vis (Spec_vis e2) k2).
 Proof.
   apply padded_refines_vis.
 Qed.
 
 Lemma padded_refines_exists_r E1 E2 R1 R2 A
-      RE REAns RR (phi : itree_spec E1 R1) (kphi : A -> itree_spec E2 R2) a :
-  padded_refines RE REAns RR phi (kphi a) ->
-  padded_refines RE REAns RR phi (Vis Spec_exists kphi).
+      RPre RPost RR (phi : itree_spec E1 R1) (kphi : A -> itree_spec E2 R2) a :
+  padded_refines RPre RPost RR phi (kphi a) ->
+  padded_refines RPre RPost RR phi (Vis Spec_exists kphi).
 Proof.
   setoid_rewrite <- bind_trigger.
   apply padded_spec_exists_elim.
 Qed.
 Lemma padded_refines_exists_l E1 E2 R1 R2 A
-      RE REAns RR (phi : itree_spec E2 R2) (kphi : A -> itree_spec E1 R1) :
-  (forall a, padded_refines RE REAns RR (kphi a) phi) ->
-  padded_refines RE REAns RR (Vis Spec_exists kphi) phi.
+      RPre RPost RR (phi : itree_spec E2 R2) (kphi : A -> itree_spec E1 R1) :
+  (forall a, padded_refines RPre RPost RR (kphi a) phi) ->
+  padded_refines RPre RPost RR (Vis Spec_exists kphi) phi.
 Proof.
   setoid_rewrite <- bind_trigger.
   apply padded_spec_exists_eliml.
 Qed.
 
 Lemma padded_refines_forall_r E1 E2 R1 R2 A
-      RE REAns RR (phi : itree_spec E1 R1) (kphi : A -> itree_spec E2 R2) :
-  (forall a, padded_refines RE REAns RR phi (kphi a)) ->
-  padded_refines RE REAns RR phi (Vis Spec_forall kphi).
+      RPre RPost RR (phi : itree_spec E1 R1) (kphi : A -> itree_spec E2 R2) :
+  (forall a, padded_refines RPre RPost RR phi (kphi a)) ->
+  padded_refines RPre RPost RR phi (Vis Spec_forall kphi).
 Proof.
   setoid_rewrite <- bind_trigger.
   apply padded_spec_forall_elim.
 Qed.
 Lemma padded_refines_forall_l E1 E2 R1 R2 A
-      RE REAns RR (phi : itree_spec E2 R2) (kphi : A -> itree_spec E1 R1) a :
-  padded_refines RE REAns RR (kphi a) phi ->
-  padded_refines RE REAns RR (Vis Spec_forall kphi) phi.
+      RPre RPost RR (phi : itree_spec E2 R2) (kphi : A -> itree_spec E1 R1) a :
+  padded_refines RPre RPost RR (kphi a) phi ->
+  padded_refines RPre RPost RR (Vis Spec_forall kphi) phi.
 Proof.
   setoid_rewrite <- bind_trigger.
   apply padded_spec_forall_eliml.
 Qed.
 
-Lemma padded_refines_if_r E1 E2 RE REAns R1 R2 RR (t1 : itree_spec E1 R1) (t2 t3: itree_spec E2 R2) b :
-  (b = true  -> padded_refines RE REAns RR t1 t2) ->
-  (b = false -> padded_refines RE REAns RR t1 t3) ->
-  padded_refines RE REAns RR t1 (if b then t2 else t3).
+Lemma padded_refines_if_r E1 E2 RPre RPost R1 R2 RR (t1 : itree_spec E1 R1) (t2 t3: itree_spec E2 R2) b :
+  (b = true  -> padded_refines RPre RPost RR t1 t2) ->
+  (b = false -> padded_refines RPre RPost RR t1 t3) ->
+  padded_refines RPre RPost RR t1 (if b then t2 else t3).
 Proof.
   intros. destruct b; eauto.
 Qed.
-Lemma padded_refines_if_l E1 E2 RE REAns R1 R2 RR (t1 t2 : itree_spec E1 R1) (t3 : itree_spec E2 R2) b :
-  (b = true  -> padded_refines RE REAns RR t1 t3) ->
-  (b = false -> padded_refines RE REAns RR t2 t3) ->
-  padded_refines RE REAns RR (if b then t1 else t2) t3.
+Lemma padded_refines_if_l E1 E2 RPre RPost R1 R2 RR (t1 t2 : itree_spec E1 R1) (t3 : itree_spec E2 R2) b :
+  (b = true  -> padded_refines RPre RPost RR t1 t3) ->
+  (b = false -> padded_refines RPre RPost RR t2 t3) ->
+  padded_refines RPre RPost RR (if b then t1 else t2) t3.
 Proof.
   intros. destruct b; eauto.
 Qed.
 
-Lemma padded_refines_if_bind_r A E1 E2 RE REAns R1 R2 RR
+Lemma padded_refines_if_bind_r A E1 E2 RPre RPost R1 R2 RR
       (t1 : itree_spec E1 R1) (t2 t3 : itree_spec E2 A)
       (t4 : A -> itree_spec E2 R2) (b : bool) :
-  padded_refines RE REAns RR t1 (if b then t2 >>= t4 else t3 >>= t4) ->
-  padded_refines RE REAns RR t1 ((if b then t2 else t3) >>= t4).
+  padded_refines RPre RPost RR t1 (if b then t2 >>= t4 else t3 >>= t4) ->
+  padded_refines RPre RPost RR t1 ((if b then t2 else t3) >>= t4).
 Proof.
   intros. destruct b; eauto.
 Qed.
-Lemma padded_refines_if_bind_l A E1 E2 RE REAns R1 R2 RR
+Lemma padded_refines_if_bind_l A E1 E2 RPre RPost R1 R2 RR
       (t1 t2 : itree_spec E1 A) (t3 : A -> itree_spec E1 R1)
       (t4 : itree_spec E2 R2) (b : bool) :
-  padded_refines RE REAns RR (if b then t1 >>= t3 else t2 >>= t3) t4 ->
-  padded_refines RE REAns RR ((if b then t1 else t2) >>= t3) t4.
+  padded_refines RPre RPost RR (if b then t1 >>= t3 else t2 >>= t3) t4 ->
+  padded_refines RPre RPost RR ((if b then t1 else t2) >>= t3) t4.
 Proof.
   intros. destruct b; eauto.
 Qed.
 
-Lemma padded_refines_match_list_r E1 E2 RE REAns R1 R2 RR A (t1 : itree_spec E1 R1)
+Lemma padded_refines_match_list_r E1 E2 RPre RPost R1 R2 RR A (t1 : itree_spec E1 R1)
       (t2 : A -> list A -> itree_spec E2 R2) (t3 : itree_spec E2 R2) xs :
-  (forall x xs', xs = x :: xs' -> padded_refines RE REAns RR t1 (t2 x xs')) ->
-  (xs = nil -> padded_refines RE REAns RR t1 t3) ->
-  padded_refines RE REAns RR t1 (match xs with | x :: xs' => t2 x xs' | nil => t3 end).
+  (forall x xs', xs = x :: xs' -> padded_refines RPre RPost RR t1 (t2 x xs')) ->
+  (xs = nil -> padded_refines RPre RPost RR t1 t3) ->
+  padded_refines RPre RPost RR t1 (match xs with | x :: xs' => t2 x xs' | nil => t3 end).
 Proof.
   intros. destruct xs; eauto.
 Qed.
-Lemma padded_refines_match_list_l E1 E2 RE REAns R1 R2 RR A (t3 : itree_spec E2 R2)
+Lemma padded_refines_match_list_l E1 E2 RPre RPost R1 R2 RR A (t3 : itree_spec E2 R2)
       (t1 : A -> list A -> itree_spec E1 R1) (t2 : itree_spec E1 R1) xs :
-  (forall x xs', xs = x :: xs' -> padded_refines RE REAns RR (t1 x xs') t3) ->
-  (xs = nil -> padded_refines RE REAns RR t2 t3) ->
-  padded_refines RE REAns RR (match xs with | x :: xs' => t1 x xs' | nil => t2 end) t3.
+  (forall x xs', xs = x :: xs' -> padded_refines RPre RPost RR (t1 x xs') t3) ->
+  (xs = nil -> padded_refines RPre RPost RR t2 t3) ->
+  padded_refines RPre RPost RR (match xs with | x :: xs' => t1 x xs' | nil => t2 end) t3.
 Proof.
   intros. destruct xs; eauto.
 Qed.
 
-Lemma padded_refines_match_list_bind_r B E1 E2 RE REAns R1 R2 RR A (t1 : itree_spec E1 R1)
+Lemma padded_refines_match_list_bind_r B E1 E2 RPre RPost R1 R2 RR A (t1 : itree_spec E1 R1)
       (t2 : A -> list A -> itree_spec E2 B) (t3 : itree_spec E2 B)
       (t4 : B -> itree_spec E2 R2) xs :
-  padded_refines RE REAns RR t1 (match xs with | x :: xs' => t2 x xs' >>= t4 | nil => t3 >>= t4 end) ->
-  padded_refines RE REAns RR t1 ((match xs with | x :: xs' => t2 x xs' | nil => t3 end) >>= t4).
+  padded_refines RPre RPost RR t1 (match xs with | x :: xs' => t2 x xs' >>= t4 | nil => t3 >>= t4 end) ->
+  padded_refines RPre RPost RR t1 ((match xs with | x :: xs' => t2 x xs' | nil => t3 end) >>= t4).
 Proof.
   intros. destruct xs; eauto.
 Qed.
-Lemma padded_refines_match_list_bind_l B E1 E2 RE REAns R1 R2 RR A (t3 : itree_spec E2 R2)
+Lemma padded_refines_match_list_bind_l B E1 E2 RPre RPost R1 R2 RR A (t3 : itree_spec E2 R2)
       (t1 : A -> list A -> itree_spec E1 B) (t2 : itree_spec E1 B)
       (t4 : B -> itree_spec E1 R1) xs :
-  padded_refines RE REAns RR (match xs with | x :: xs' => t1 x xs' >>= t4 | nil => t2 >>= t4 end) t3 ->
-  padded_refines RE REAns RR ((match xs with | x :: xs' => t1 x xs' | nil => t2 end) >>= t4) t3.
+  padded_refines RPre RPost RR (match xs with | x :: xs' => t1 x xs' >>= t4 | nil => t2 >>= t4 end) t3 ->
+  padded_refines RPre RPost RR ((match xs with | x :: xs' => t1 x xs' | nil => t2 end) >>= t4) t3.
 Proof.
   intros. destruct xs; eauto.
 Qed.
 
-Lemma padded_refines_match_pair_r E1 E2 RE REAns R1 R2 RR A B
+Lemma padded_refines_match_pair_r E1 E2 RPre RPost R1 R2 RR A B
       (t1 : itree_spec E1 R1) (t2 : A -> B -> itree_spec E2 R2) pr :
-  (forall x y, pr = (x, y) -> padded_refines RE REAns RR t1 (t2 x y)) ->
-  padded_refines RE REAns RR t1 (match pr with | (x,y) => t2 x y end).
+  (forall x y, pr = (x, y) -> padded_refines RPre RPost RR t1 (t2 x y)) ->
+  padded_refines RPre RPost RR t1 (match pr with | (x,y) => t2 x y end).
 Proof.
   intros. destruct pr; eauto.
 Qed.
-Lemma padded_refines_match_pair_l E1 E2 RE REAns R1 R2 RR A B
+Lemma padded_refines_match_pair_l E1 E2 RPre RPost R1 R2 RR A B
       (t1 : A -> B -> itree_spec E1 R1) (t2 : itree_spec E2 R2) pr :
-  (forall x y, pr = (x, y) -> padded_refines RE REAns RR (t1 x y) t2) ->
-  padded_refines RE REAns RR (match pr with | (x,y) => t1 x y end) t2.
+  (forall x y, pr = (x, y) -> padded_refines RPre RPost RR (t1 x y) t2) ->
+  padded_refines RPre RPost RR (match pr with | (x,y) => t1 x y end) t2.
 Proof.
   intros. destruct pr; eauto.
 Qed.
 
-Lemma padded_refines_match_pair_bind_r C E1 E2 RE REAns R1 R2 RR A B
+Lemma padded_refines_match_pair_bind_r C E1 E2 RPre RPost R1 R2 RR A B
       (t1 : itree_spec E1 R1) (t2 : A -> B -> itree_spec E2 C)
       (t3 : C -> itree_spec E2 R2) pr :
-  padded_refines RE REAns RR t1 (match pr with | (x,y) => t2 x y >>= t3 end) ->
-  padded_refines RE REAns RR t1 ((match pr with | (x,y) => t2 x y end) >>= t3).
+  padded_refines RPre RPost RR t1 (match pr with | (x,y) => t2 x y >>= t3 end) ->
+  padded_refines RPre RPost RR t1 ((match pr with | (x,y) => t2 x y end) >>= t3).
 Proof.
   intros. destruct pr; eauto.
 Qed.
-Lemma padded_refines_match_pair_bind_l C E1 E2 RE REAns R1 R2 RR A B
+Lemma padded_refines_match_pair_bind_l C E1 E2 RPre RPost R1 R2 RR A B
       (t1 : A -> B -> itree_spec E1 C) (t2 : itree_spec E2 R2)
       (t3 : C -> itree_spec E1 R1) pr :
-  padded_refines RE REAns RR (match pr with | (x,y) => t1 x y >>= t3 end) t2 ->
-  padded_refines RE REAns RR ((match pr with | (x,y) => t1 x y end) >>= t3) t2.
+  padded_refines RPre RPost RR (match pr with | (x,y) => t1 x y >>= t3 end) t2 ->
+  padded_refines RPre RPost RR ((match pr with | (x,y) => t1 x y end) >>= t3) t2.
 Proof.
   intros. destruct pr; eauto.
 Qed.
 
 Lemma padded_refines_ret_bind_r E1 E2 R1 R2 A
-      RE REAns RR (phi : itree_spec E1 R1) r (kphi : A -> itree_spec E2 R2) :
-  padded_refines RE REAns RR phi (kphi r) ->
-  padded_refines RE REAns RR phi (Ret r >>= kphi).
+      RPre RPost RR (phi : itree_spec E1 R1) r (kphi : A -> itree_spec E2 R2) :
+  padded_refines RPre RPost RR phi (kphi r) ->
+  padded_refines RPre RPost RR phi (Ret r >>= kphi).
 Proof.
   setoid_rewrite bind_ret_l; eauto.
 Qed.
 Lemma padded_refines_ret_bind_l E1 E2 R1 R2 A
-      RE REAns RR (phi : itree_spec E2 R2) r (kphi : A -> itree_spec E1 R1) :
-  padded_refines RE REAns RR (kphi r) phi ->
-  padded_refines RE REAns RR (Ret r >>= kphi) phi.
+      RPre RPost RR (phi : itree_spec E2 R2) r (kphi : A -> itree_spec E1 R1) :
+  padded_refines RPre RPost RR (kphi r) phi ->
+  padded_refines RPre RPost RR (Ret r >>= kphi) phi.
 Proof.
   setoid_rewrite bind_ret_l; eauto.
 Qed.
 
 Lemma padded_refines_trigger_bind_r E1 E2 R1 R2 A
-      RE REAns RR (phi : itree_spec E1 R1) e (kphi : A -> itree_spec E2 R2) :
-  padded_refines RE REAns RR phi (Vis e kphi) ->
-  padded_refines RE REAns RR phi (ITree.trigger e >>= kphi).
+      RPre RPost RR (phi : itree_spec E1 R1) e (kphi : A -> itree_spec E2 R2) :
+  padded_refines RPre RPost RR phi (Vis e kphi) ->
+  padded_refines RPre RPost RR phi (ITree.trigger e >>= kphi).
 Proof.
   setoid_rewrite bind_trigger; eauto.
 Qed.
 Lemma padded_refines_trigger_bind_l E1 E2 R1 R2 A
-      RE REAns RR (phi : itree_spec E2 R2) e (kphi : A -> itree_spec E1 R1) :
-  padded_refines RE REAns RR (Vis e kphi) phi ->
-  padded_refines RE REAns RR (ITree.trigger e >>= kphi) phi.
+      RPre RPost RR (phi : itree_spec E2 R2) e (kphi : A -> itree_spec E1 R1) :
+  padded_refines RPre RPost RR (Vis e kphi) phi ->
+  padded_refines RPre RPost RR (ITree.trigger e >>= kphi) phi.
 Proof.
   setoid_rewrite bind_trigger; eauto.
 Qed.
 
 Lemma padded_refines_vis_bind_r E1 E2 R1 R2 A1 A2
-      RE REAns RR (phi : itree_spec E1 R1) e
+      RPre RPost RR (phi : itree_spec E1 R1) e
       (kphi1 : A1 -> itree_spec E2 A2) (kphi2 : A2 -> itree_spec E2 R2) :
-  padded_refines RE REAns RR phi (Vis e (fun a => kphi1 a >>= kphi2)) ->
-  padded_refines RE REAns RR phi (Vis e kphi1 >>= kphi2).
+  padded_refines RPre RPost RR phi (Vis e (fun a => kphi1 a >>= kphi2)) ->
+  padded_refines RPre RPost RR phi (Vis e kphi1 >>= kphi2).
 Proof.
   setoid_rewrite bind_vis; eauto.
 Qed.
 Lemma padded_refines_vis_bind_l E1 E2 R1 R2 A1 A2
-      RE REAns RR (phi : itree_spec E2 R2) e
+      RPre RPost RR (phi : itree_spec E2 R2) e
       (kphi1 : A1 -> itree_spec E1 A2) (kphi2 : A2 -> itree_spec E1 R1) :
-  padded_refines RE REAns RR (Vis e (fun a => kphi1 a >>= kphi2)) phi ->
-  padded_refines RE REAns RR (Vis e kphi1 >>= kphi2) phi.
+  padded_refines RPre RPost RR (Vis e (fun a => kphi1 a >>= kphi2)) phi ->
+  padded_refines RPre RPost RR (Vis e kphi1 >>= kphi2) phi.
 Proof.
   setoid_rewrite bind_vis; eauto.
 Qed.
 
 Lemma padded_refines_bind_bind_r E1 E2 R1 R2 A1 A2
-      RE REAns RR (phi1 : itree_spec E1 R1) (phi2 : itree_spec E2 A1)
+      RPre RPost RR (phi1 : itree_spec E1 R1) (phi2 : itree_spec E2 A1)
       (kphi1 : A1 -> itree_spec E2 A2) (kphi2 : A2 -> itree_spec E2 R2) :
-  padded_refines RE REAns RR phi1 (phi2 >>= (fun a => kphi1 a >>= kphi2)) ->
-  padded_refines RE REAns RR phi1 ((phi2 >>= kphi1) >>= kphi2).
+  padded_refines RPre RPost RR phi1 (phi2 >>= (fun a => kphi1 a >>= kphi2)) ->
+  padded_refines RPre RPost RR phi1 ((phi2 >>= kphi1) >>= kphi2).
 Proof.
   setoid_rewrite bind_bind; eauto.
 Qed.
 Lemma padded_refines_bind_bind_l E1 E2 R1 R2 A1 A2
-      RE REAns RR (phi1 : itree_spec E2 A1) (phi2 : itree_spec E1 R1)
+      RPre RPost RR (phi1 : itree_spec E2 A1) (phi2 : itree_spec E1 R1)
       (kphi1 : A1 -> itree_spec E2 A2) (kphi2 : A2 -> itree_spec E2 R2) :
-  padded_refines RE REAns RR (phi1 >>= (fun a => kphi1 a >>= kphi2)) phi2 ->
-  padded_refines RE REAns RR ((phi1 >>= kphi1) >>= kphi2) phi2.
+  padded_refines RPre RPost RR (phi1 >>= (fun a => kphi1 a >>= kphi2)) phi2 ->
+  padded_refines RPre RPost RR ((phi1 >>= kphi1) >>= kphi2) phi2.
 Proof.
   setoid_rewrite bind_bind; eauto.
 Qed.
@@ -232,18 +232,18 @@ Qed.
 Section Rec.
 
 Context (E1 E2 : Type -> Type) (A1 A2 R1 R2 : Type).
-Context (RE : PreRel E1 E2) (REAns : PostRel E1 E2) (RR : R1 -> R2 -> Prop).
+Context (RPre : PreRel E1 E2) (RPost : PostRel E1 E2) (RR : R1 -> R2 -> Prop).
 
 Context (precond : A1 -> A2 -> Prop)
         (postcond : forall a1 a2, precond a1 a2 -> forall r1 r2, RR r1 r2 -> Prop).
 
-Variant padded_refines_rec_REInv : PreRel (callE A1 R1) (callE A2 R2) :=
-  | padded_refines_rec_REInv_i a1 a2 : precond a1 a2 ->
-    padded_refines_rec_REInv R1 R2 (Call a1) (Call a2).
+Variant padded_refines_rec_RPreInv : PreRel (callE A1 R1) (callE A2 R2) :=
+  | padded_refines_rec_RPreInv_i a1 a2 : precond a1 a2 ->
+    padded_refines_rec_RPreInv R1 R2 (Call a1) (Call a2).
 
-Variant padded_refines_rec_REAnsInv : PostRel (callE A1 R1) (callE A2 R2) :=
-  | padded_refines_rec_REAnsInv_i a1 a2 r1 r2 p : depProdRel RR (postcond a1 a2 p) r1 r2 ->
-    padded_refines_rec_REAnsInv R1 R2 (Call a1) (Call a2) r1 r2.
+Variant padded_refines_rec_RPostInv : PostRel (callE A1 R1) (callE A2 R2) :=
+  | padded_refines_rec_RPostInv_i a1 a2 r1 r2 p : depProdRel RR (postcond a1 a2 p) r1 r2 ->
+    padded_refines_rec_RPostInv R1 R2 (Call a1) (Call a2) r1 r2.
 
 Context (body1 : A1 -> itree_spec (callE A1 R1 +' E1) R1).
 
@@ -253,19 +253,19 @@ Context (body2 : A2 -> itree_spec (callE A2 R2 +' E2) R2).
 Lemma padded_refines_rec (a1 : A1) (a2 : A2) :
   precond a1 a2 ->
   (forall a1 a2 (p : precond a1 a2),
-     padded_refines (sumPreRel padded_refines_rec_REInv RE)
-                    (sumPostRel padded_refines_rec_REAnsInv REAns)
+     padded_refines (sumPreRel padded_refines_rec_RPreInv RPre)
+                    (sumPostRel padded_refines_rec_RPostInv RPost)
                     (depProdRel RR (postcond a1 a2 p))
                     (body1 a1) (body2 a2)) ->
-  padded_refines RE REAns RR (mrec_spec (calling' body1) (Call a1))
+  padded_refines RPre RPost RR (mrec_spec (calling' body1) (Call a1))
                              (mrec_spec (calling' body2) (Call a2)).
 Proof.
   intros.
   eapply padded_refines_monot with
-    (RR1 := padded_refines_rec_REAnsInv R1 R2 (Call a1) (Call a2)); eauto.
+    (RR1 := padded_refines_rec_RPostInv R1 R2 (Call a1) (Call a2)); eauto.
   { intros. inv PR. destruct H7. inj_existT. subst. auto. }
-  eapply padded_refines_mrec with (REInv := padded_refines_rec_REInv)
-                                  (REAnsInv := padded_refines_rec_REAnsInv).
+  eapply padded_refines_mrec with (RPreInv := padded_refines_rec_RPreInv)
+                                  (RPostInv := padded_refines_rec_RPostInv).
   - intros A B [] [] []. unfold calling'.
     eapply padded_refines_monot with (RR1 := depProdRel RR (postcond a3 a4 H1)); eauto.
     intros. econstructor; eauto.
@@ -291,11 +291,11 @@ Lemma padded_refines_total_spec (a1 : A1) (a2 : A2) :
   well_founded rdec ->
   precond a1 a2 ->
   (forall a1 a2 (p : precond a1 a2),
-     padded_refines (sumPreRel padded_refines_rec_REInv RE)
-                    (sumPostRel padded_refines_rec_REAnsInv REAns)
+     padded_refines (sumPreRel padded_refines_rec_RPreInv RPre)
+                    (sumPostRel padded_refines_rec_RPostInv RPost)
                     (depProdRel RR (postcond a1 a2 p))
                     (body1 a1) (total_spec_fix_body a2)) ->
-  padded_refines RE REAns RR (mrec_spec (calling' body1) (Call a1))
+  padded_refines RPre RPost RR (mrec_spec (calling' body1) (Call a1))
                              (total_spec Pre Post a2).
 Proof.
   intro; rewrite <- total_spec_fix_total; eauto.
@@ -304,28 +304,28 @@ Qed.
 
 End Rec.
 
-Lemma padded_refines_trepeat_zero_r E1 E2 R1 R2 RE REAns RR
+Lemma padded_refines_trepeat_zero_r E1 E2 R1 R2 RPre RPost RR
       (t1 : itree_spec E1 R1) (t2 : itree_spec E2 R2) :
-  padded_refines RE REAns RR t1 (Ret tt) ->
-  padded_refines RE REAns RR t1 (trepeat 0 t2).
+  padded_refines RPre RPost RR t1 (Ret tt) ->
+  padded_refines RPre RPost RR t1 (trepeat 0 t2).
 Proof. eauto. Qed.
 
-Lemma padded_refines_trepeat_suc_r E1 E2 R1 R2 RE REAns RR
+Lemma padded_refines_trepeat_suc_r E1 E2 R1 R2 RPre RPost RR
       (t1 : itree_spec E1 R1) n (t2 : itree_spec E2 R2) :
-  padded_refines RE REAns RR t1 (t2 ;; trepeat n t2) ->
-  padded_refines RE REAns RR t1 (trepeat (S n) t2).
+  padded_refines RPre RPost RR t1 (t2 ;; trepeat n t2) ->
+  padded_refines RPre RPost RR t1 (trepeat (S n) t2).
 Proof. eauto. Qed.
 
-Lemma padded_refines_trepeat_bind_zero_r E1 E2 R1 R2 R3 RE REAns RR
+Lemma padded_refines_trepeat_bind_zero_r E1 E2 R1 R2 R3 RPre RPost RR
       (t1 : itree_spec E1 R1) (t2 : itree_spec E2 R2) (t3 : unit -> itree_spec E2 R3) :
-  padded_refines RE REAns RR t1 (t3 tt) ->
-  padded_refines RE REAns RR t1 (trepeat 0 t2 >>= t3).
+  padded_refines RPre RPost RR t1 (t3 tt) ->
+  padded_refines RPre RPost RR t1 (trepeat 0 t2 >>= t3).
 Proof. eauto. Qed.
 
-Lemma padded_refines_trepeat_bind_suc_r E1 E2 R1 R2 R3 RE REAns RR
+Lemma padded_refines_trepeat_bind_suc_r E1 E2 R1 R2 R3 RPre RPost RR
       (t1 : itree_spec E1 R1) n (t2 : itree_spec E2 R2) (t3 : unit -> itree_spec E2 R3) :
-  padded_refines RE REAns RR t1 (t2 ;; (trepeat n t2 >>= t3)) ->
-  padded_refines RE REAns RR t1 (trepeat (S n) t2 >>= t3).
+  padded_refines RPre RPost RR t1 (t2 ;; (trepeat n t2 >>= t3)) ->
+  padded_refines RPre RPost RR t1 (trepeat (S n) t2 >>= t3).
 Proof. simpl; rewrite bind_bind; eauto. Qed.
 
 
@@ -390,29 +390,29 @@ Polymorphic Lemma IntroArg_and n P Q (goal : P /\ Q -> Prop)
 Proof. intros H [ p q ]; apply H. Qed.
 
 Polymorphic Lemma IntroArg_sumPreRel_inl n E1 E2 F1 F2
-                  (REE : PreRel E1 E2) (REF : PreRel F1 F2)
+                  (RPreE : PreRel E1 E2) (RPreF : PreRel F1 F2)
                   A B e1 e2 (goal : _ -> Prop) :
-  IntroArg n (REE A B e1 e2) (fun p => goal (sumPreRel_inl _ _ _ _ _ _ p)) ->
-  IntroArg n (@sumPreRel E1 E2 F1 F2 REE REF A B (inl1 e1) (inl1 e2)) goal.
+  IntroArg n (RPreE A B e1 e2) (fun p => goal (sumPreRel_inl _ _ _ _ _ _ p)) ->
+  IntroArg n (@sumPreRel E1 E2 F1 F2 RPreE RPreF A B (inl1 e1) (inl1 e2)) goal.
 Proof. intros ?H ?H; dependent destruction H0; apply H. Qed.
 Polymorphic Lemma IntroArg_sumPreRel_inr n E1 E2 F1 F2
-                  (REE : PreRel E1 E2) (REF : PreRel F1 F2)
+                  (RPreE : PreRel E1 E2) (RPreF : PreRel F1 F2)
                   A B f1 f2 (goal : _ -> Prop) :
-  IntroArg n (REF A B f1 f2) (fun p => goal (sumPreRel_inr _ _ _ _ _ _ p)) ->
-  IntroArg n (@sumPreRel E1 E2 F1 F2 REE REF A B (inr1 f1) (inr1 f2)) goal.
+  IntroArg n (RPreF A B f1 f2) (fun p => goal (sumPreRel_inr _ _ _ _ _ _ p)) ->
+  IntroArg n (@sumPreRel E1 E2 F1 F2 RPreE RPreF A B (inr1 f1) (inr1 f2)) goal.
 Proof. intros ?H ?H; dependent destruction H0; apply H. Qed.
 
 Polymorphic Lemma IntroArg_sumPostRel_inl n E1 E2 F1 F2
-                  (REE : PostRel E1 E2) (REF : PostRel F1 F2)
+                  (RPreE : PostRel E1 E2) (RPreF : PostRel F1 F2)
                   A B e1 e2 a b (goal : _ -> Prop) :
-  IntroArg n (REE A B e1 e2 a b) (fun p => goal (sumPostRel_inl _ _ _ _ _ _ _ _ p)) ->
-  IntroArg n (@sumPostRel E1 E2 F1 F2 REE REF A B (inl1 e1) (inl1 e2) a b) goal.
+  IntroArg n (RPreE A B e1 e2 a b) (fun p => goal (sumPostRel_inl _ _ _ _ _ _ _ _ p)) ->
+  IntroArg n (@sumPostRel E1 E2 F1 F2 RPreE RPreF A B (inl1 e1) (inl1 e2) a b) goal.
 Proof. intros ?H ?H; dependent destruction H0; apply H. Qed.
 Polymorphic Lemma IntroArg_sumPostRel_inr n E1 E2 F1 F2
-                  (REE : PostRel E1 E2) (REF : PostRel F1 F2)
+                  (RPreE : PostRel E1 E2) (RPreF : PostRel F1 F2)
                   A B f1 f2 a b (goal : _ -> Prop) :
-  IntroArg n (REF A B f1 f2 a b) (fun p => goal (sumPostRel_inr _ _ _ _ _ _ _ _ p)) ->
-  IntroArg n (@sumPostRel E1 E2 F1 F2 REE REF A B (inr1 f1) (inr1 f2) a b) goal.
+  IntroArg n (RPreF A B f1 f2 a b) (fun p => goal (sumPostRel_inr _ _ _ _ _ _ _ _ p)) ->
+  IntroArg n (@sumPostRel E1 E2 F1 F2 RPreE RPreF A B (inr1 f1) (inr1 f2) a b) goal.
 Proof. intros ?H ?H; dependent destruction H0; apply H. Qed.
 
 Polymorphic Lemma IntroArg_eqPostRel n E A e a1 a2 (goal : _ -> Prop) :
@@ -424,20 +424,20 @@ Proof.
   erewrite eq_rect_eq; eauto.
 Qed.
 
-Polymorphic Lemma IntroArg_padded_refines_rec_REInv_i n A1 A2 R1 R2
+Polymorphic Lemma IntroArg_padded_refines_rec_RPreInv_i n A1 A2 R1 R2
                   (precond : A1 -> A2 -> Prop) a1 a2 (goal : _ -> Prop) :
-  IntroArg n (precond a1 a2) (fun p => goal (padded_refines_rec_REInv_i _ _ _ _ _ _ _ p)) ->
-  IntroArg n (padded_refines_rec_REInv A1 A2 R1 R2 precond R1 R2 (Call a1) (Call a2)) goal.
+  IntroArg n (precond a1 a2) (fun p => goal (padded_refines_rec_RPreInv_i _ _ _ _ _ _ _ p)) ->
+  IntroArg n (padded_refines_rec_RPreInv A1 A2 R1 R2 precond R1 R2 (Call a1) (Call a2)) goal.
 Proof. intros ?H ?H; dependent destruction H0; apply H. Qed.
 
-Polymorphic Lemma IntroArg_padded_refines_rec_REAnsInv_i n A1 A2 R1 R2
+Polymorphic Lemma IntroArg_padded_refines_rec_RPostInv_i n A1 A2 R1 R2
                   (RR : R1 -> R2 -> Prop) (precond : A1 -> A2 -> Prop)
                   (postcond : forall a1 a2, precond a1 a2 -> forall (r1 : R1) (r2 : R2), RR r1 r2 -> Prop)
                   a1 a2 r1 r2 (goal : _ -> Prop) :
   IntroArg n (precond a1 a2) (fun p0 => IntroArg n (RR r1 r2) (fun p1 =>
   IntroArg n (postcond a1 a2 p0 r1 r2 p1) (fun p2 =>
-    goal (padded_refines_rec_REAnsInv_i _ _ _ _ _ _ _ _ _ _ _ p0 (exist _ p1 p2))))) ->
-  IntroArg n (padded_refines_rec_REAnsInv A1 A2 R1 R2 RR precond postcond R1 R2 (Call a1) (Call a2) r1 r2) goal.
+    goal (padded_refines_rec_RPostInv_i _ _ _ _ _ _ _ _ _ _ _ p0 (exist _ p1 p2))))) ->
+  IntroArg n (padded_refines_rec_RPostInv A1 A2 R1 R2 RR precond postcond R1 R2 (Call a1) (Call a2) r1 r2) goal.
 Proof. intros ?H ?H; dependent destruction H0; dependent destruction d; apply H. Qed.
 
 Ltac IntroArg_intro_dependent_destruction n :=
@@ -481,8 +481,8 @@ Ltac IntroArg_base_tac n A g :=
   | sumPostRel _ _ _ _ (ReSum_inr _ _ _ _ _ _ _) (inl1 _) _ _ => IntroArg_intro_dependent_destruction n
   | sumPostRel _ _ _ _ (ReSum_inr _ _ _ _ _ _ _) (ReSum_inl _ _ _ _ _ _ _) _ _ => IntroArg_intro_dependent_destruction n
   | eqPostRel _ _ _ _ _ _ => apply IntroArg_eqPostRel
-  | padded_refines_rec_REInv _ _ _ _ _ _ _ (Call _) (Call _) => simple apply IntroArg_padded_refines_rec_REInv_i
-  | padded_refines_rec_REAnsInv _ _ _ _ _ _ _ _ _ (Call _) (Call _) _ _ => simple apply IntroArg_padded_refines_rec_REAnsInv_i
+  | padded_refines_rec_RPreInv _ _ _ _ _ _ _ (Call _) (Call _) => simple apply IntroArg_padded_refines_rec_RPreInv_i
+  | padded_refines_rec_RPostInv _ _ _ _ _ _ _ _ _ (Call _) (Call _) _ _ => simple apply IntroArg_padded_refines_rec_RPostInv_i
   | true  = true  => IntroArg_intro_dependent_destruction n
   | false = false => IntroArg_intro_dependent_destruction n
   | true  = false => IntroArg_intro_dependent_destruction n
@@ -511,15 +511,15 @@ Proof. eauto. Qed.
 Hint Extern 101 (RelGoal ((fun _ => _) _)) =>
   simple apply RelGoal_eta.
 
-Lemma RelGoal_sumPreRel_inl E1 E2 F1 F2 (REE : PreRel E1 E2) (REF : PreRel F1 F2)
+Lemma RelGoal_sumPreRel_inl E1 E2 F1 F2 (RPreE : PreRel E1 E2) (RPreF : PreRel F1 F2)
                            A B e1 e2 :
-  RelGoal (REE A B e1 e2) ->
-  RelGoal (@sumPreRel E1 E2 F1 F2 REE REF A B (inl1 e1) (inl1 e2)).
+  RelGoal (RPreE A B e1 e2) ->
+  RelGoal (@sumPreRel E1 E2 F1 F2 RPreE RPreF A B (inl1 e1) (inl1 e2)).
 Proof. constructor; eauto. Qed.
-Lemma RelGoal_sumPreRel_inr E1 E2 F1 F2 (REE : PreRel E1 E2) (REF : PreRel F1 F2)
+Lemma RelGoal_sumPreRel_inr E1 E2 F1 F2 (RPreE : PreRel E1 E2) (RPreF : PreRel F1 F2)
                            A B f1 f2 :
-  RelGoal (REF A B f1 f2) ->
-  RelGoal (@sumPreRel E1 E2 F1 F2 REE REF A B (inr1 f1) (inr1 f2)).
+  RelGoal (RPreF A B f1 f2) ->
+  RelGoal (@sumPreRel E1 E2 F1 F2 RPreE RPreF A B (inr1 f1) (inr1 f2)).
 Proof. constructor; eauto. Qed.
 
 Hint Extern 101 (RelGoal (sumPreRel _ _ _ _ (inl1 _) (inl1 _))) =>
@@ -539,15 +539,15 @@ Hint Extern 101 (RelGoal (sumPreRel _ _ _ _ (ReSum_inr _ _ _ _ _ _ _) (inr1 _)))
 Hint Extern 101 (RelGoal (sumPreRel _ _ _ _ (ReSum_inr _ _ _ _ _ _ _) (ReSum_inr _ _ _ _ _ _ _))) =>
   apply RelGoal_sumPreRel_inr : refines.
 
-Lemma RelGoal_sumPostRel_inl E1 E2 F1 F2 (REE : PostRel E1 E2) (REF : PostRel F1 F2)
+Lemma RelGoal_sumPostRel_inl E1 E2 F1 F2 (RPreE : PostRel E1 E2) (RPreF : PostRel F1 F2)
                               A B e1 e2 a b :
-  RelGoal (REE A B e1 e2 a b) ->
-  RelGoal (@sumPostRel E1 E2 F1 F2 REE REF A B (inl1 e1) (inl1 e2) a b).
+  RelGoal (RPreE A B e1 e2 a b) ->
+  RelGoal (@sumPostRel E1 E2 F1 F2 RPreE RPreF A B (inl1 e1) (inl1 e2) a b).
 Proof. constructor; eauto. Qed.
-Lemma RelGoal_sumPostRel_inr E1 E2 F1 F2 (REE : PostRel E1 E2) (REF : PostRel F1 F2)
+Lemma RelGoal_sumPostRel_inr E1 E2 F1 F2 (RPreE : PostRel E1 E2) (RPreF : PostRel F1 F2)
                               A B f1 f2 a b :
-  RelGoal (REF A B f1 f2 a b) ->
-  RelGoal (@sumPostRel E1 E2 F1 F2 REE REF A B (inr1 f1) (inr1 f2) a b).
+  RelGoal (RPreF A B f1 f2 a b) ->
+  RelGoal (@sumPostRel E1 E2 F1 F2 RPreE RPreF A B (inr1 f1) (inr1 f2) a b).
 Proof. constructor; eauto. Qed.
 
 Hint Extern 101 (RelGoal (sumPostRel _ _ _ _ (inl1 _) (inl1 _) _ _)) =>
@@ -567,26 +567,26 @@ Hint Extern 101 (RelGoal (sumPostRel _ _ _ _ (ReSum_inr _ _ _ _ _ _ _) (inr1 _) 
 Hint Extern 101 (RelGoal (sumPostRel _ _ _ _ (ReSum_inr _ _ _ _ _ _ _) (ReSum_inr _ _ _ _ _ _ _) _ _)) =>
   apply RelGoal_sumPostRel_inr : refines.
 
-Lemma RelGoal_padded_refines_rec_REInv_i A1 A2 R1 R2
+Lemma RelGoal_padded_refines_rec_RPreInv_i A1 A2 R1 R2
       (precond : A1 -> A2 -> Prop)  a1 a2 :
   RelGoal (precond a1 a2) ->
-  RelGoal (padded_refines_rec_REInv A1 A2 R1 R2 precond R1 R2 (Call a1) (Call a2)).
+  RelGoal (padded_refines_rec_RPreInv A1 A2 R1 R2 precond R1 R2 (Call a1) (Call a2)).
 Proof. constructor; eauto. Qed.
 
-Hint Extern 101 (RelGoal (padded_refines_rec_REInv _ _ _ _ _ _ _ (Call _) (Call _))) =>
-  simple apply RelGoal_padded_refines_rec_REInv_i : refines.
+Hint Extern 101 (RelGoal (padded_refines_rec_RPreInv _ _ _ _ _ _ _ (Call _) (Call _))) =>
+  simple apply RelGoal_padded_refines_rec_RPreInv_i : refines.
 
-Lemma RelGoal_padded_refines_rec_REAnsInv_i A1 A2 R1 R2
+Lemma RelGoal_padded_refines_rec_RPostInv_i A1 A2 R1 R2
       (RR : R1 -> R2 -> Prop) (precond : A1 -> A2 -> Prop)
       (postcond : forall a1 a2, precond a1 a2 -> forall (r1 : R1) (r2 : R2), RR r1 r2 -> Prop)
       a1 a2 r1 r2 :
   forall (p0 : RelGoal (precond a1 a2)) (p1 : RelGoal (RR r1 r2)),
   RelGoal (postcond a1 a2 p0 r1 r2 p1) ->
-  RelGoal (padded_refines_rec_REAnsInv A1 A2 R1 R2 RR precond postcond R1 R2 (Call a1) (Call a2) r1 r2).
+  RelGoal (padded_refines_rec_RPostInv A1 A2 R1 R2 RR precond postcond R1 R2 (Call a1) (Call a2) r1 r2).
 Proof. econstructor; econstructor; eauto. Qed.
 
-Hint Extern 101 (RelGoal (padded_refines_rec_REAnsInv _ _ _ _ _ _ _ _ _ (Call _) (Call _) _ _)) =>
-  simple apply RelGoal_padded_refines_rec_REAnsInv_i : refines.
+Hint Extern 101 (RelGoal (padded_refines_rec_RPostInv _ _ _ _ _ _ _ _ _ (Call _) (Call _) _ _)) =>
+  simple apply RelGoal_padded_refines_rec_RPostInv_i : refines.
 
 Lemma RelGoal_depProdRel {R1 R2} (RR1 : R1 -> R2 -> Prop) (RR2 : forall r1 r2, RR1 r1 r2 -> Prop) r1 r2 :
   forall (p1 : RelGoal (RR1 r1 r2)), RelGoal (RR2 r1 r2 p1) ->
@@ -606,23 +606,23 @@ Hint Extern 101 (RelGoal (eqPreRel _ _ _ _)) =>
 
 (** * Basic Refinement Hints *)
 
-Definition padded_refines_ret_IntroArg E1 E2 R1 R2 RE REAns RR r1 r2 :
+Definition padded_refines_ret_IntroArg E1 E2 R1 R2 RPre RPost RR r1 r2 :
   (RelGoal (RR r1 r2 : Prop)) ->
-  @padded_refines E1 E2 R1 R2 RE REAns RR (Ret r1) (Ret r2) :=
-  padded_refines_ret E1 E2 R1 R2 RE REAns RR r1 r2.
+  @padded_refines E1 E2 R1 R2 RPre RPost RR (Ret r1) (Ret r2) :=
+  padded_refines_ret E1 E2 R1 R2 RPre RPost RR r1 r2.
 
 Hint Extern 102 (padded_refines _ _ _ (Ret _) (Ret _)) =>
   apply padded_refines_ret_IntroArg : refines.
 
 Definition padded_refines_vis_IntroArg E1 E2 R1 R2 A B
-        RE REAns RR (e1 : E1 A) (e2 : E2 B)
+        RPre RPost RR (e1 : E1 A) (e2 : E2 B)
         (k1 : A -> itree_spec E1 R1) (k2 : B -> itree_spec E2 R2) :
-  (RelGoal (RE A B e1 e2 : Prop)) ->
+  (RelGoal (RPre A B e1 e2 : Prop)) ->
   (IntroArg Any A (fun a => IntroArg Any B (fun b =>
-     IntroArg Hyp (REAns A B e1 e2 a b : Prop) (fun _ =>
-       padded_refines RE REAns RR (k1 a) (k2 b))))) ->
-  padded_refines RE REAns RR (Vis (Spec_vis e1) k1) (Vis (Spec_vis e2) k2) :=
-  padded_refines_vis E1 E2 R1 R2 A B RE REAns RR e1 e2 k1 k2.
+     IntroArg Hyp (RPost A B e1 e2 a b : Prop) (fun _ =>
+       padded_refines RPre RPost RR (k1 a) (k2 b))))) ->
+  padded_refines RPre RPost RR (Vis (Spec_vis e1) k1) (Vis (Spec_vis e2) k2) :=
+  padded_refines_vis E1 E2 R1 R2 A B RPre RPost RR e1 e2 k1 k2.
 
 Hint Extern 102 (padded_refines _ _ _ (Vis (Spec_vis _) _) (Vis (Spec_vis _) _)) =>
   apply padded_refines_vis_IntroArg : refines.
@@ -636,15 +636,15 @@ Hint Extern 103 (padded_refines _ _ _ (vis _ _) (vis _ _)) =>
   apply padded_refines_vis_IntroArg : refines.
 
 Definition padded_refines_exists_l_IntroArg E1 E2 R1 R2 A
-      RE REAns RR (phi : itree_spec E2 R2) (kphi : A -> itree_spec E1 R1) :
-  (IntroArg Exists A (fun a => padded_refines RE REAns RR (kphi a) phi)) ->
-  padded_refines RE REAns RR (Vis Spec_exists kphi) phi :=
-  padded_refines_exists_l E1 E2 R1 R2 A RE REAns RR phi kphi.
+      RPre RPost RR (phi : itree_spec E2 R2) (kphi : A -> itree_spec E1 R1) :
+  (IntroArg Exists A (fun a => padded_refines RPre RPost RR (kphi a) phi)) ->
+  padded_refines RPre RPost RR (Vis Spec_exists kphi) phi :=
+  padded_refines_exists_l E1 E2 R1 R2 A RPre RPost RR phi kphi.
 Definition padded_refines_forall_r_IntroArg E1 E2 R1 R2 A
-      RE REAns RR (phi : itree_spec E1 R1) (kphi : A -> itree_spec E2 R2) :
-  (IntroArg Forall A (fun a => padded_refines RE REAns RR phi (kphi a))) ->
-  padded_refines RE REAns RR phi (Vis Spec_forall kphi) :=
-  padded_refines_forall_r E1 E2 R1 R2 A RE REAns RR phi kphi.
+      RPre RPost RR (phi : itree_spec E1 R1) (kphi : A -> itree_spec E2 R2) :
+  (IntroArg Forall A (fun a => padded_refines RPre RPost RR phi (kphi a))) ->
+  padded_refines RPre RPost RR phi (Vis Spec_forall kphi) :=
+  padded_refines_forall_r E1 E2 R1 R2 A RPre RPost RR phi kphi.
 
 Hint Extern 101 (padded_refines _ _ _ _ (Vis Spec_forall _)) =>
   simple apply padded_refines_forall_r_IntroArg : refines.
@@ -664,16 +664,16 @@ Hint Extern 102 (padded_refines _ _ _ (Vis Spec_forall _) _) =>
 Hint Extern 102 (padded_refines _ _ _ (vis Spec_forall _) _) =>
   unshelve (eapply padded_refines_forall_l); [shelve|] : refines.
 
-Definition padded_refines_if_r_IntroArg E1 E2 RE REAns R1 R2 RR t1 t2 t3 b :
-  (IntroArg If (b = true) (fun _ => padded_refines RE REAns RR t1 t2)) ->
-  (IntroArg If (b = false) (fun _ => padded_refines RE REAns RR t1 t3)) ->
-  padded_refines RE REAns RR t1 (if b then t2 else t3) :=
-  padded_refines_if_r E1 E2 RE REAns R1 R2 RR t1 t2 t3 b.
-Definition padded_refines_if_l_IntroArg E1 E2 RE REAns R1 R2 RR t1 t2 t3 b :
-  (IntroArg If (b = true) (fun _ => padded_refines RE REAns RR t1 t3)) ->
-  (IntroArg If (b = false) (fun _ => padded_refines RE REAns RR t2 t3)) ->
-  padded_refines RE REAns RR (if b then t1 else t2) t3 :=
-  padded_refines_if_l E1 E2 RE REAns R1 R2 RR t1 t2 t3 b.
+Definition padded_refines_if_r_IntroArg E1 E2 RPre RPost R1 R2 RR t1 t2 t3 b :
+  (IntroArg If (b = true) (fun _ => padded_refines RPre RPost RR t1 t2)) ->
+  (IntroArg If (b = false) (fun _ => padded_refines RPre RPost RR t1 t3)) ->
+  padded_refines RPre RPost RR t1 (if b then t2 else t3) :=
+  padded_refines_if_r E1 E2 RPre RPost R1 R2 RR t1 t2 t3 b.
+Definition padded_refines_if_l_IntroArg E1 E2 RPre RPost R1 R2 RR t1 t2 t3 b :
+  (IntroArg If (b = true) (fun _ => padded_refines RPre RPost RR t1 t3)) ->
+  (IntroArg If (b = false) (fun _ => padded_refines RPre RPost RR t2 t3)) ->
+  padded_refines RPre RPost RR (if b then t1 else t2) t3 :=
+  padded_refines_if_l E1 E2 RPre RPost R1 R2 RR t1 t2 t3 b.
 
 Hint Extern 101 (padded_refines _ _ _ _ (if _ then _ else _)) =>
   apply padded_refines_if_r_IntroArg : refines.
@@ -685,20 +685,20 @@ Hint Extern 101 (padded_refines _ _ _ _ ((if _ then _ else _) >>= _)) =>
 Hint Extern 101 (padded_refines _ _ _ ((if _ then _ else _) >>= _) _) =>
   apply padded_refines_if_bind_l : refines.
 
-Definition padded_refines_match_list_r_IntroArg E1 E2 RE REAns R1 R2 RR A (t1 : itree_spec E1 R1)
+Definition padded_refines_match_list_r_IntroArg E1 E2 RPre RPost R1 R2 RR A (t1 : itree_spec E1 R1)
       (t2 : A -> list A -> itree_spec E2 R2) (t3 : itree_spec E2 R2) xs :
   (IntroArg Any A (fun x => IntroArg Any (list A) (fun xs' =>
-   IntroArg Match (xs = x :: xs') (fun _ => padded_refines RE REAns RR t1 (t2 x xs'))))) ->
-  (IntroArg Match (xs = nil) (fun _ => padded_refines RE REAns RR t1 t3)) ->
-  padded_refines RE REAns RR t1 (match xs with | x :: xs' => t2 x xs' | nil => t3 end) :=
-  padded_refines_match_list_r E1 E2 RE REAns R1 R2 RR A t1 t2 t3 xs.
-Definition padded_refines_match_list_l_IntroArg E1 E2 RE REAns R1 R2 RR A (t3 : itree_spec E2 R2)
+   IntroArg Match (xs = x :: xs') (fun _ => padded_refines RPre RPost RR t1 (t2 x xs'))))) ->
+  (IntroArg Match (xs = nil) (fun _ => padded_refines RPre RPost RR t1 t3)) ->
+  padded_refines RPre RPost RR t1 (match xs with | x :: xs' => t2 x xs' | nil => t3 end) :=
+  padded_refines_match_list_r E1 E2 RPre RPost R1 R2 RR A t1 t2 t3 xs.
+Definition padded_refines_match_list_l_IntroArg E1 E2 RPre RPost R1 R2 RR A (t3 : itree_spec E2 R2)
       (t1 : A -> list A -> itree_spec E1 R1) (t2 : itree_spec E1 R1) xs :
   (IntroArg Any A (fun x => IntroArg Any (list A) (fun xs' =>
-   IntroArg Match (xs = x :: xs') (fun _ => padded_refines RE REAns RR (t1 x xs') t3)))) ->
-  (IntroArg Match (xs = nil) (fun _ => padded_refines RE REAns RR t2 t3)) ->
-  padded_refines RE REAns RR (match xs with | x :: xs' => t1 x xs' | nil => t2 end) t3 :=
-  padded_refines_match_list_l E1 E2 RE REAns R1 R2 RR A t3 t1 t2 xs.
+   IntroArg Match (xs = x :: xs') (fun _ => padded_refines RPre RPost RR (t1 x xs') t3)))) ->
+  (IntroArg Match (xs = nil) (fun _ => padded_refines RPre RPost RR t2 t3)) ->
+  padded_refines RPre RPost RR (match xs with | x :: xs' => t1 x xs' | nil => t2 end) t3 :=
+  padded_refines_match_list_l E1 E2 RPre RPost R1 R2 RR A t3 t1 t2 xs.
 
 Hint Extern 101 (padded_refines _ _ _ _ (match _ with | _ :: _ => _ | nil => _ end)) =>
   apply padded_refines_match_list_r_IntroArg : refines.
@@ -710,18 +710,18 @@ Hint Extern 101 (padded_refines _ _ _ _ ((match _ with | _ :: _ => _ | nil => _ 
 Hint Extern 101 (padded_refines _ _ _ ((match _ with | _ :: _ => _ | nil => _ end) >>= _) _) =>
   apply padded_refines_match_list_bind_l : refines.
 
-Definition padded_refines_match_pair_r_IntroArg E1 E2 RE REAns R1 R2 RR A B
+Definition padded_refines_match_pair_r_IntroArg E1 E2 RPre RPost R1 R2 RR A B
       (t1 : itree_spec E1 R1) (t2 : A -> B -> itree_spec E2 R2) pr :
   (IntroArg Any A (fun x => IntroArg Any B (fun y =>
-   IntroArg Match (pr = (x, y)) (fun _ => padded_refines RE REAns RR t1 (t2 x y))))) ->
-  padded_refines RE REAns RR t1 (match pr with | (x,y) => t2 x y end) :=
-  padded_refines_match_pair_r E1 E2 RE REAns R1 R2 RR A B t1 t2 pr.
-Definition padded_refines_match_pair_l_IntroArg E1 E2 RE REAns R1 R2 RR A B
+   IntroArg Match (pr = (x, y)) (fun _ => padded_refines RPre RPost RR t1 (t2 x y))))) ->
+  padded_refines RPre RPost RR t1 (match pr with | (x,y) => t2 x y end) :=
+  padded_refines_match_pair_r E1 E2 RPre RPost R1 R2 RR A B t1 t2 pr.
+Definition padded_refines_match_pair_l_IntroArg E1 E2 RPre RPost R1 R2 RR A B
       (t1 : A -> B -> itree_spec E1 R1) (t2 : itree_spec E2 R2) pr :
   (IntroArg Any A (fun x => IntroArg Any B (fun y =>
-   IntroArg Match (pr = (x, y)) (fun _ => padded_refines RE REAns RR (t1 x y) t2)))) ->
-  padded_refines RE REAns RR (match pr with | (x,y) => t1 x y end) t2 :=
-  padded_refines_match_pair_l E1 E2 RE REAns R1 R2 RR A B t1 t2 pr.
+   IntroArg Match (pr = (x, y)) (fun _ => padded_refines RPre RPost RR (t1 x y) t2)))) ->
+  padded_refines RPre RPost RR (match pr with | (x,y) => t1 x y end) t2 :=
+  padded_refines_match_pair_l E1 E2 RPre RPost R1 R2 RR A B t1 t2 pr.
 
 Hint Extern 101 (padded_refines _ _ _ _ (match _ with | (_,_) => _ end)) =>
   apply padded_refines_match_pair_r_IntroArg : refines.
@@ -757,13 +757,13 @@ Hint Extern 101 (padded_refines _ _ _ _ ((_ >>= _) >>= _)) =>
 Hint Extern 101 (padded_refines _ _ _ ((_ >>= _) >>= _) _) =>
   simple apply padded_refines_bind_bind_l : refines.
 
-Definition padded_refines_trigger_r E1 E2 R1 R2 RE REAns RR phi e :
-  padded_refines RE REAns RR phi (Vis e (fun x => Ret x)) ->
-  @padded_refines E1 E2 R1 R2 RE REAns RR phi (ITree.trigger e) :=
+Definition padded_refines_trigger_r E1 E2 R1 R2 RPre RPost RR phi e :
+  padded_refines RPre RPost RR phi (Vis e (fun x => Ret x)) ->
+  @padded_refines E1 E2 R1 R2 RPre RPost RR phi (ITree.trigger e) :=
   fun r => r.
-Definition padded_refines_trigger_l E1 E2 R1 R2 RE REAns RR phi e :
-  padded_refines RE REAns RR (Vis e (fun x => Ret x)) phi ->
-  @padded_refines E1 E2 R1 R2 RE REAns RR (ITree.trigger e) phi :=
+Definition padded_refines_trigger_l E1 E2 R1 R2 RPre RPost RR phi e :
+  padded_refines RPre RPost RR (Vis e (fun x => Ret x)) phi ->
+  @padded_refines E1 E2 R1 R2 RPre RPost RR (ITree.trigger e) phi :=
   fun r => r.
 
 Hint Extern 101 (padded_refines _ _ _ _ (ITree.trigger _)) =>
@@ -837,7 +837,7 @@ Hint Extern 999 (well_founded _) => shelve : refines.
 Hint Extern 999 (Continue _ _) => shelve : refines.
 
 Definition padded_refines_rec_IntroArg
-           E1 E2 A1 A2 R1 R2 RE REAns (RR : R1 -> R2 -> Prop) body1 body2 a1 a2
+           E1 E2 A1 A2 R1 R2 RPre RPost (RR : R1 -> R2 -> Prop) body1 body2 a1 a2
            (precond : IntroArg Any A1 (fun a1 => IntroArg Any A2 (fun a2 => Precondition a1 a2)))
            (postcond : IntroArg Any A1 (fun a1 => IntroArg Any A2 (fun a2 =>
                        IntroArg Hyp (precond a1 a2) (fun H =>
@@ -846,14 +846,14 @@ Definition padded_refines_rec_IntroArg
   Continue (precond a1 a2)
            (IntroArg Any A1 (fun a1 => IntroArg Any A2 (fun a2 =>
             IntroArg Hyp (precond a1 a2) (fun p =>
-            padded_refines (sumPreRel _ RE)
-                           (sumPostRel _ REAns)
+            padded_refines (sumPreRel _ RPre)
+                           (sumPostRel _ RPost)
                            (depProdRel RR (postcond a1 a2 p))
                            (body1 a1) (body2 a2))))) ->
-  padded_refines RE REAns RR (mrec_spec (calling' body1) (Call a1))
+  padded_refines RPre RPost RR (mrec_spec (calling' body1) (Call a1))
                              (mrec_spec (calling' body2) (Call a2)) := fun pr =>
   match pr with
-  | (p, q) => padded_refines_rec E1 E2 A1 A2 R1 R2 RE REAns RR precond postcond body1 body2 a1 a2 p q
+  | (p, q) => padded_refines_rec E1 E2 A1 A2 R1 R2 RPre RPost RR precond postcond body1 body2 a1 a2 p q
   end.
 
 Ltac padded_refines_rec := eapply padded_refines_rec_IntroArg.
@@ -867,7 +867,7 @@ Hint Extern 101 (padded_refines _ _ _ (rec_fix_spec _ _) (rec_fix_spec _ _)) =>
   padded_refines_rec : refines.
 
 Definition padded_refines_total_spec_IntroArg
-           E1 E2 A1 A2 R1 R2 RE REAns (RR : R1 -> R2 -> Prop) body1 a1 a2 Pre Post
+           E1 E2 A1 A2 R1 R2 RPre RPost (RR : R1 -> R2 -> Prop) body1 a1 a2 Pre Post
            (precond : IntroArg Any A1 (fun a1 => IntroArg Any A2 (fun a2 => Precondition a1 a2)))
            (postcond : IntroArg Any A1 (fun a1 => IntroArg Any A2 (fun a2 =>
                        IntroArg Hyp (precond a1 a2) (fun H =>
@@ -878,14 +878,14 @@ Definition padded_refines_total_spec_IntroArg
   Continue (precond a1 a2)
            (IntroArg Any A1 (fun a1 => IntroArg Any A2 (fun a2 =>
             IntroArg Hyp (precond a1 a2) (fun p =>
-            padded_refines (sumPreRel _ RE)
-                           (sumPostRel _ REAns)
+            padded_refines (sumPreRel _ RPre)
+                           (sumPostRel _ RPost)
                            (depProdRel RR (postcond a1 a2 p))
                            (body1 a1) (total_spec_fix_body _ _ _ Pre Post rdec a2))))) ->
-  padded_refines RE REAns RR (mrec_spec (calling' body1) (Call a1))
+  padded_refines RPre RPost RR (mrec_spec (calling' body1) (Call a1))
                              (total_spec Pre Post a2) := fun pf pr =>
   match pr with
-  | (p, q) => padded_refines_total_spec E1 E2 A1 A2 R1 R2 RE REAns RR precond postcond body1 Pre Post rdec a1 a2 pf p q
+  | (p, q) => padded_refines_total_spec E1 E2 A1 A2 R1 R2 RPre RPost RR precond postcond body1 Pre Post rdec a1 a2 pf p q
   end.
 
 Ltac padded_refines_total_spec :=
