theories/HeterogeneousEventRelations.v
@@ -12,47 +12,47 @@ Definition depProdRel {A B} (RR1 : Rel A B)
 Notation PreRel E1 E2 := (forall (A B : Type), (E1 A : Type) -> (E2 B : Type) -> Prop).
 
 (*this is stronger than we need *)
-Class ReflexivePreRel {E : Type -> Type} (RE : PreRel E E) : Prop :=
-  reflexivePreRel : forall A (e : E A), RE A A e e.
+Class ReflexivePreRel {E : Type -> Type} (RPre : PreRel E E) : Prop :=
+  reflexivePreRel : forall A (e : E A), RPre A A e e.
 
-Class SymmetricPreRel {E : Type -> Type} (RE : PreRel E E) : Prop :=
-  symmetricPreRel : forall A B (e1 : E A) (e2 : E B), RE A B e1 e2 -> RE B A e2 e1.
+Class SymmetricPreRel {E : Type -> Type} (RPre : PreRel E E) : Prop :=
+  symmetricPreRel : forall A B (e1 : E A) (e2 : E B), RPre A B e1 e2 -> RPre B A e2 e1.
 
-Class TransitivePreRel {E : Type -> Type} (RE : PreRel E E) : Prop :=
+Class TransitivePreRel {E : Type -> Type} (RPre : PreRel E E) : Prop :=
   transitivePreRel : forall A B C (e1 : E A) (e2 : E B) (e3 : E C),
-    RE A B e1 e2 -> RE B C e2 e3 -> RE A C e1 e3.
+    RPre A B e1 e2 -> RPre B C e2 e3 -> RPre A C e1 e3.
 
-Definition flipPreRel {E1 E2 : Type -> Type} (RE : PreRel E1 E2) : PreRel E2 E1 :=
-  fun A B e1 e2 => RE B A e2 e1.
+Definition flipPreRel {E1 E2 : Type -> Type} (RPre : PreRel E1 E2) : PreRel E2 E1 :=
+  fun A B e1 e2 => RPre B A e2 e1.
 
 Variant rcomposePreRel {E1 E2 E3 : Type -> Type}
-           (RE12 : PreRel E1 E2) (RE23 : PreRel E2 E3) : forall A C, E1 A -> E3 C -> Prop :=
-  rcomposePreRel_intro (A B C: Type) e1 e2 e3 : RE12 A B e1 e2 -> RE23 B C e2 e3 -> rcomposePreRel RE12 RE23 A C e1 e3.
+           (RPre12 : PreRel E1 E2) (RPre23 : PreRel E2 E3) : forall A C, E1 A -> E3 C -> Prop :=
+  rcomposePreRel_intro (A B C: Type) e1 e2 e3 : RPre12 A B e1 e2 -> RPre23 B C e2 e3 -> rcomposePreRel RPre12 RPre23 A C e1 e3.
 
-Variant sumPreRel {E1 E2 F1 F2} (REE : PreRel E1 E2) (REF : PreRel F1 F2) : forall A B, (E1 +' F1) A -> (E2 +' F2) B -> Prop :=
-| sumPreRel_inl A B (e1 : E1 A) (e2 : E2 B) : REE A B e1 e2 -> sumPreRel REE REF A B (inl1 e1) (inl1 e2)
-| sumPreRel_inr A B (f1 : F1 A) (f2 : F2 B) : REF A B f1 f2 -> sumPreRel REE REF A B (inr1 f1) (inr1 f2).
+Variant sumPreRel {E1 E2 F1 F2} (RPreE : PreRel E1 E2) (RPreF : PreRel F1 F2) : forall A B, (E1 +' F1) A -> (E2 +' F2) B -> Prop :=
+| sumPreRel_inl A B (e1 : E1 A) (e2 : E2 B) : RPreE A B e1 e2 -> sumPreRel RPreE RPreF A B (inl1 e1) (inl1 e2)
+| sumPreRel_inr A B (f1 : F1 A) (f2 : F2 B) : RPreF A B f1 f2 -> sumPreRel RPreE RPreF A B (inr1 f1) (inr1 f2).
 
 
 Notation PostRel E1 E2 := (forall (A B : Type), (E1 A : Type) -> (E2 B : Type) -> A -> B -> Prop).
 
-Variant sumPostRel {E1 E2 F1 F2} (REE : PostRel E1 E2) (REF : PostRel F1 F2) :
+Variant sumPostRel {E1 E2 F1 F2} (RPreE : PostRel E1 E2) (RPreF : PostRel F1 F2) :
   forall A B, (E1 +' F1) A -> (E2 +' F2) B -> A -> B -> Prop :=
-| sumPostRel_inl A B (e1 : E1 A) (e2 : E2 B) a b : REE A B e1 e2 a b -> sumPostRel REE REF A B (inl1 e1) (inl1 e2) a b
-| sumPostRel_inr A B (f1 : F1 A) (f2 : F2 B) a b : REF A B f1 f2 a b -> sumPostRel REE REF A B (inr1 f1) (inr1 f2) a b
+| sumPostRel_inl A B (e1 : E1 A) (e2 : E2 B) a b : RPreE A B e1 e2 a b -> sumPostRel RPreE RPreF A B (inl1 e1) (inl1 e2) a b
+| sumPostRel_inr A B (f1 : F1 A) (f2 : F2 B) a b : RPreF A B f1 f2 a b -> sumPostRel RPreE RPreF A B (inr1 f1) (inr1 f2) a b
 .
 
 (* This may need to be defined in dependent on two PreRel's?*)
 (*
 Variant rcomposePostRel' {E1 E2 E3 : Type -> Type}
-           (RE12 : PostRel E1 E2) (RE23 : PostRel E2 E3):
+           (RPre12 : PostRel E1 E2) (RPre23 : PostRel E2 E3):
   forall A C, E1 A -> E3 C -> A -> C -> Prop :=
   | rcomposePostRel_intro (A B C : Type)
                        (*maybe I should somehow universally quantify this*)
                        (e1 : E1 A) (e2 : E2 B) (e3 : E3 C)
                        a b c :
-    RE12 A B e1 e2 a b -> RE23 B C e2 e3 b c ->
-    rcomposePostRel RE12 RE23 A C e1 e3 a c.
+    RPre12 A B e1 e2 a b -> RPre23 B C e2 e3 b c ->
+    rcomposePostRel RPre12 RPre23 A C e1 e3 a c.
 *)
 
 
@@ -62,27 +62,27 @@ Variant rcomposePostRel' {E1 E2 E3 : Type -> Type}
    a new case for this possibility
  *)
 Variant rcomposePostRel {E1 E2 E3 : Type -> Type}
-           (RE12 : PostRel E1 E2) (RE23 : PostRel E2 E3)
-           (RE : forall A B C, E1 A -> E2 B -> E3 C -> Prop)
+           (RPre12 : PostRel E1 E2) (RPre23 : PostRel E2 E3)
+           (RPre : forall A B C, E1 A -> E2 B -> E3 C -> Prop)
   :
   forall A C, E1 A -> E3 C -> A -> C -> Prop :=
   | rcomposePostRel_intro (A C : Type)
                        (e1 : E1 A) (e3 : E3 C)
                        a c :
     (forall B (e2 : E2 B),
-      RE A B C e1 e2 e3 -> exists b, RE12 A B e1 e2 a b /\ RE23 B C e2 e3 b c) ->
-    rcomposePostRel RE12 RE23 RE A C e1 e3 a c.
+      RPre A B C e1 e2 e3 -> exists b, RPre12 A B e1 e2 a b /\ RPre23 B C e2 e3 b c) ->
+    rcomposePostRel RPre12 RPre23 RPre A C e1 e3 a c.
 
 (*this is stronger than I need*)
-(* I see 2 ways to do it, either it is reflexive wrt RE
+(* I see 2 ways to do it, either it is reflexive wrt RPre
    or *)
-Class ReflexivePostRel {E : Type -> Type} (REA : PostRel E E) : Prop :=
+Class ReflexivePostRel {E : Type -> Type} (RPreA : PostRel E E) : Prop :=
   reflexivePostRel : forall A (e : E A) (a b : A),
-      REA A A e e a b -> a = b.
+      RPreA A A e e a b -> a = b.
 
-Class SymmetricPostRel {E : Type -> Type} (REA : PostRel E E) : Prop :=
+Class SymmetricPostRel {E : Type -> Type} (RPreA : PostRel E E) : Prop :=
   symmetricPostRel : forall A B (e1 : E A) (e2 : E B) a b,
-      REA A B e1 e2 a b -> REA B A e2 e1 b a.
+      RPreA A B e1 e2 a b -> RPreA B A e2 e1 b a.
 
 
 Variant eqPreRel {E} : PreRel E E :=
